trans.v
@@ -1,6 +1,9 @@
 From istari Require Import Sigma Tactics
      Syntax Subst SimpSub Promote Hygiene
      ContextHygiene Equivalence Rules Defined.
-From istari Require Import help.
+From istari Require Import source subst_src rules_src help.
 
-(*trans_type: (term False) -> ((term False) -> (term False)) -> type.*)
+Inductive trans_type: (source.term False) -> (Syntax.term False) -> Type :=
+  tt_ref: forall A As, trans_type A As -> trans_type (reftp_m A) (make_ref As).
+
+Inductive trans
